src/Ast/StaticConsistency.dfy
@@ -1,0 +1,218 @@
+module StaticConsistency {
+  import opened Std.Wrappers
+  import opened Basics
+  import opened Ast
+
+  method CheckConsistent(program: Program) returns (outcome: Outcome<string>)
+    requires program.WellFormed()
+    ensures outcome.Pass? ==> Consistent(program)
+  {
+    var procs := program.procedures;
+    while procs != {}
+      invariant forall proc :: proc in program.procedures - procs ==> ConsistentProc(proc)
+    {
+      var proc :| proc in procs;
+      procs := procs - {proc};
+      :- CheckProcedure(proc);
+    }
+    return Pass;
+  }
+
+  predicate Consistent(b3: Program)
+    requires b3.WellFormed()
+    reads b3.procedures
+  {
+    forall proc <- b3.procedures :: ConsistentProc(proc)
+  }
+
+  predicate ConsistentProc(proc: Procedure)
+    requires proc.WellFormed()
+    reads proc
+  {
+    && (forall ae <- proc.Pre :: ConsistentAExpr(ae))
+    && (forall ae <- proc.Post :: ConsistentAExpr(ae))
+    && (proc.Body.Some? ==> ConsistentStmt(proc.Body.value))
+  }
+
+  predicate ConsistentAExpr(aexpr: AExpr)
+    requires aexpr.WellFormed()
+  {
+    match aexpr
+    case AExpr(e) => true
+    case AAssertion(s) =>
+      ConsistentStmt(s) && !ContainsNonAssertions(s)
+  }
+
+  predicate ConsistentStmt(stmt: Stmt)
+    requires stmt.WellFormed()
+  {
+    match stmt
+    case VarDecl(_, _, body) =>
+      ConsistentStmt(body)
+    case Assign(lhs, rhs) =>
+      lhs.IsMutable()
+    case Block(stmts) =>
+      forall s <- stmts :: ConsistentStmt(s)
+    case Call(proc, args) =>
+      forall i :: 0 <= i < |args| ==> proc.Parameters[i].mode == args[i].CorrespondingMode()
+    case Check(cond) => true
+    case Assume(cond) => true
+    case Assert(cond) => true
+    case AForall(_, body) =>
+      ConsistentStmt(body) && !ContainsNonAssertions(body)
+    case If(cases) =>
+      forall c <- cases :: ConsistentStmt(c.body)
+    case Loop(invariants, body) =>
+      && (forall inv <- invariants :: ConsistentAExpr(inv))
+      && ConsistentStmt(body)
+    case LabeledStmt(_, body) =>
+      ConsistentStmt(body)
+    case Exit(_) => true
+    case Probe(expr) => true
+  }
+
+  predicate ContainsNonAssertions(stmt: Stmt) {
+    match stmt
+    case VarDecl(v, _, body) =>
+      v.IsMutable() || ContainsNonAssertions(body)
+    case Assign(_, _) => true
+    case Block(stmts) =>
+      exists stmt <- stmts :: ContainsNonAssertions(stmt)
+    case Call(_, _) => true
+    case Check(_) => false
+    case Assume(_) => false
+    case Assert(_) => false
+    case AForall(_, body) =>
+      ContainsNonAssertions(body)
+    case If(cases) =>
+      exists cs <- cases :: ContainsNonAssertions(cs.body)
+    case Loop(_, _) => true
+    case LabeledStmt(_, _) => true
+    case Exit(_) => true
+    case Probe(_) => false
+  }
+
+  method CheckProcedure(proc: Procedure) returns (outcome: Outcome<string>)
+    requires proc.WellFormed()
+    ensures outcome.Pass? ==> ConsistentProc(proc)
+  {
+    for n := 0 to |proc.Pre|
+      invariant forall ae <- proc.Pre[..n] :: ConsistentAExpr(ae)
+    {
+      :- CheckAExpr(proc.Pre[n]);
+    }
+    for n := 0 to |proc.Post|
+      invariant forall ae <- proc.Post[..n] :: ConsistentAExpr(ae)
+    {
+      :- CheckAExpr(proc.Post[n]);
+    }
+    if proc.Body.Some? {
+      :- CheckStmt(proc.Body.value);
+    }
+    return Pass;
+  }
+
+  method CheckAExpr(aexpr: AExpr) returns (outcome: Outcome<string>)
+    requires aexpr.WellFormed()
+    ensures outcome.Pass? ==> ConsistentAExpr(aexpr)
+  {
+    match aexpr
+    case AExpr(_) =>
+      return Pass;
+    case AAssertion(s) =>
+      :- CheckStmt(s);
+      :- CheckCanBeUsedInAssertion(s);
+      return Pass;
+  }
+
+  method CheckStmt(stmt: Stmt) returns (outcome: Outcome<string>)
+    requires stmt.WellFormed()
+    ensures outcome.Pass? ==> ConsistentStmt(stmt)
+  {
+    match stmt {
+      case VarDecl(_, _, body) =>
+        :- CheckStmt(body);
+      case Assign(lhs, _) =>
+        if !lhs.IsMutable() {
+          return Fail("assignment to immutable variable '" + lhs.name + "'");
+        }
+      case Block(stmts) =>
+        for n := 0 to |stmts|
+          invariant forall stmt <- stmts[..n] :: ConsistentStmt(stmt)
+        {
+          :- CheckStmt(stmts[n]);
+        }
+      case Call(proc, args) =>
+        for n := 0 to |args|
+          invariant forall i :: 0 <= i < n ==> proc.Parameters[i].mode == args[i].CorrespondingMode()
+        {
+          var formal := proc.Parameters[n];
+          var actual := args[n];
+          if formal.mode != actual.CorrespondingMode() {
+            var a := formal.mode.ToString();
+            var b := actual.CorrespondingMode().ToString();
+            return Fail("incorrect parameter mode; expected " + a + "-parameter, got " + b + "-parameter");
+          }
+        }
+      case Check(_) =>
+      case Assume(_) =>
+      case Assert(_) =>
+      case AForall(_, body) =>
+        :- CheckStmt(body);
+        if ContainsNonAssertions(body) {
+          return Fail("'forall' statement is not allowed to contain non-assertions");
+        }
+      case If(cases) =>
+        for n := 0 to |cases|
+          invariant forall cs <- cases[..n] :: ConsistentStmt(cs.body)
+        {
+          :- CheckStmt(cases[n].body);
+        }
+      case Loop(invariants, body) =>
+        for n := 0 to |invariants|
+          invariant forall inv <- invariants[..n] :: ConsistentAExpr(inv)
+        {
+          :- CheckAExpr(invariants[n]);
+        }
+        :- CheckStmt(body);
+      case LabeledStmt(_, body) =>
+        :- CheckStmt(body);
+      case Exit(_) =>
+      case Probe(_) =>
+    }
+    return Pass;
+  }
+
+  method CheckCanBeUsedInAssertion(stmt: Stmt) returns (outcome: Outcome<string>)
+    ensures outcome.Pass? ==> !ContainsNonAssertions(stmt)
+  {
+    match stmt {
+      case VarDecl(v, _, body) =>
+        if v.IsMutable() {
+          return Fail("assertion is allowed to declare a mutable variable: '" + v.name + "'");
+        }
+        :- CheckCanBeUsedInAssertion(body);
+      case Block(stmts) =>
+        for n := 0 to |stmts|
+          invariant forall stmt <- stmts[..n] :: !ContainsNonAssertions(stmt)
+        {
+          :- CheckCanBeUsedInAssertion(stmts[n]);
+        }
+      case Check(_) =>
+      case Assume(_) =>
+      case Assert(_) =>
+      case AForall(_, body) =>
+        :- CheckCanBeUsedInAssertion(body);
+      case If(cases) =>
+        for n := 0 to |cases|
+          invariant forall cs <- cases[..n] :: !ContainsNonAssertions(cs.body)
+        {
+          :- CheckCanBeUsedInAssertion(cases[n].body);
+        }
+      case Probe(_) =>
+      case _ =>
+        return Fail("assertion can only contain assertion-compatible statements");
+    }
+    return Pass;
+  }
+}
